Some advances on delimited release : wallet verifies
* but almost everything else seems out of reach

examples/rel/delimitedReleaseReify.fst
@@ -54,7 +54,6 @@ type del_rel (i:int) (env:env) (vl:list id{List.length vl = i}) (ihel:list iexpr
 
 reifiable
 val test : prog 3
-reifiable
 let test [x;y;z] =
   let tmp1 = read y in
   let tmp2 = read z in
@@ -74,55 +73,85 @@ val verify_test (x y z: id):
 let verify_test x y z = ()
 
 reifiable
+val sum4 : prog 4
+let sum4 [y ; x1 ; x2 ; x3 ] =
+  write y (read x1 + read x2 + read x3 )
+
+val verify_sum4 (x1 x2 x3 y : id):
+  Lemma begin
+    let n = 4  in
+    let l = [x1 ; x2 ; x3 ] in
+    assert_norm (List.length l == n - 1) ;
+    let env : env = fun r ->
+      (* expanding the definition of mem here seems faster to verify *)
+      if List.mem r l then High else Low
+    in
+    let sum4_val h = fst (reify (read x1 + read x2 + read x3 ) h) in
+    del_rel n env (y::l) [sum4_val] [] sum4
+  end
+let verify_sum4 x1 x2 x3 y = ()
+
+
+(* Starting from a sum with 5 variables you need to modify the rlimit *)
+#set-options "--z3rlimit 100"
+
+reifiable
 val sum : prog 6
 let sum [y ; x1 ; x2 ; x3 ; x4 ; x5] =
   write y (read x1 + read x2 + read x3 + read x4 + read x5)
-  (* upd h y ((sel h x1 + sel h x2 + sel h x3 + sel h x4 + sel h x5)) *)
 
 (* The variant with 4 variables seems to work... *)
-(* val verify_sum (x1 x2 x3 x4 x5 y : id): *)
+val verify_sum (x1 x2 x3 x4 x5 y : id):
+  Lemma begin
+    let n = 6 in
+    let l = [x1 ; x2 ; x3 ; x4 ; x5] in
+    let env : env = fun r ->
+      (* expanding the definition of mem here seems faster to verify *)
+      if List.mem r l then High else Low
+    in
+    let sum_val h = fst (reify (read x1 + read x2 + read x3 + read x4 + read x5) h) in
+    del_rel n env (y::l) [sum_val] [] sum
+  end
+let verify_sum x1 x2 x3 x4 x5 y = ()
+
+#set-options "--z3rlimit 5"
+
+(* Does not verify !!! *)
+
+(* reifiable *)
+(* val sum_swap : prog 6 *)
+(* let sum_swap [y ; x1 ; x2 ; x3 ; x4 ; x5] = *)
+(*   let tmp1 = read x1 in *)
+(*   write x1 (read x2) ; *)
+(*   write x2 (read x3) ; *)
+(*   write x3 (read x4) ; *)
+(*   write x4 (read x5) ; *)
+(*   write x5 tmp1 ; *)
+(*   write y (read x1 + read x2 + read x3 + read x4 + read x5) *)
+
+(* val verify_sum_swap (x1 x2 x3 x4 x5 y : id): *)
 (*   Lemma begin *)
 (*     let n = 6 in *)
-(*     let l = [x1 ; x2 ; x3 ; x4 ; x5] in *)
+(*     let l = [x1;x2;x3;x4;x5] in *)
 (*     let env : env = fun r -> *)
-(*       if r = x1 || r = x2 || r = x3 || r = x4 || r = x5 then High else Low *)
+(*       if List.mem r l then High *)
+(*       else Low *)
 (*     in *)
 (*     let sum_val h = fst (reify (read x1 + read x2 + read x3 + read x4 + read x5) h) in *)
-(*     del_rel n env (y::l) [sum_val] [] sum *)
+(*     del_rel n env (y::l) [sum_val] [] sum_swap *)
 (*   end *)
-(* let verify_sum x1 x2 x3 x4 x5 y = () *)
-
-(* val sum_swap : prog 6 *)
-(* let sum_swap [x1;x2;x3;x4;x5;y] h = *)
-(*   let tmp1 = sel h x1 in *)
-(*   let h = upd h x1 (sel h x2) in *)
-(*   let h = upd h x2 (sel h x3) in *)
-(*   let h = upd h x3 (sel h x4) in *)
-(*   let h = upd h x4 (sel h x5) in *)
-(*   let h = upd h x5 tmp1 in *)
-(*   upd h y ((sel h x1 + sel h x2 + sel h x3 + sel h x4 + sel h x5)) *)
-
-(* val verify_sum_swap (x1 x2 x3 x4 x5 y : ref int): *)
-(*   Lemma *)
-(*     (del_rel 6 *)
-(*       (fun r -> *)
-(*         if r = y then Low *)
-(*         else if List.mem r [x1;x2;x3;x4;x5] then High *)
-(*         else Low) *)
-(*       [x1;x2;x3;x4;x5;y] *)
-(*       [fun h -> sel h x1 + sel h x2 + sel h x3 + sel h x4 + sel h x5] *)
-(*       [] *)
-(*       sum_swap) *)
 (* let verify_sum_swap x1 x2 x3 x4 x5 y = () *)
 
-(* val sum_att : prog 6 *)
-(* let sum_att [x1;x2;x3;x4;x5;y] h = *)
-(*   let tmp1 = sel h x1 in *)
-(*   let h = upd h x2 tmp1 in *)
-(*   let h = upd h x3 tmp1 in *)
-(*   let h = upd h x4 tmp1 in *)
-(*   let h = upd h x5 tmp1 in *)
-(*   upd h y ((sel h x1 + sel h x2 + sel h x3 + sel h x4 + sel h x5)) *)
+
+reifiable
+val sum_att : prog 6
+let sum_att [y ; x1 ; x2 ; x3 ; x4 ; x5] =
+  let tmp1 = read x1 in
+  write x2 tmp1 ;
+  write x3 tmp1 ;
+  write x4 tmp1 ;
+  write x5 tmp1 ;
+  write y ((read x1 + read x2 + read x3 + read x4 + read x5))
 
 (* (\* This does not verify, as expected *\) *)
 (* (\* *)
@@ -140,38 +169,48 @@ let sum [y ; x1 ; x2 ; x3 ; x4 ; x5] =
 (* *\) *)
 
 
-(* val wallet : prog 3 *)
-(* let wallet [x_h;k;x_l] h = *)
-(*   if (sel h x_h >= sel h k) then *)
-(*     let h = upd h x_h (sel h x_h - sel h k) in *)
-(*     let h = upd h x_l (sel h x_l + sel h k) in *)
-(*     h *)
-(*   else *)
-(*     h *)
+#set-options "--z3rlimit 100"
+reifiable
+val wallet : prog 3
+let wallet [x_h ; k ; x_l] =
+  if (read x_h >= read k) then
+    write x_h (read x_h - read k) ;
+    write x_l (read x_l + read k)
 
-(* val verify_wallet (x_h k x_l : ref int): *)
-(*   Lemma *)
-(*     (del_rel 3 *)
-(*       (fun r -> *)
-(*         if r = x_h then High *)
-(*         else Low) *)
-(*       [x_h; k; x_l] *)
-(*       [] *)
-(*       [fun h -> sel h x_h >= sel h k] *)
-(*       wallet) *)
-(* let verify_wallet x_h k x_l = () *)
+val verify_wallet (x_h k x_l : id):
+  Lemma begin
+    let n = 3 in
+    let env : env = fun r -> if r = x_h then High else Low in
+    let l = [x_h ; k ; x_l] in
+    let b h = fst (reify (read x_h >= read k) h) in
+    del_rel n env l [] [b] wallet
+  end
+let verify_wallet x_h k x_l = ()
 
-(* // This is not accepted *)
-(* //val wallet_attack_loop : prog 4 *)
-(* val wallet_attack_loop : vl:list(ref int){List.length vl = 4 /\ List.noRepeats vl} -> h:heap -> GTot heap (decreases (sel h (List.hd vl))) *)
-(* let rec wallet_attack_loop [n;x_h;k;x_l] h = *)
-(*   if sel h n <= 0 then *)
-(*     h *)
-(*   else *)
-(*     let h = upd h k (pow2 (sel h n - 1)) in *)
-(*     let h = wallet [x_h;k;x_l] h in *)
-(*     let h = upd h n (sel h n - 1) in *)
-(*     wallet_attack_loop [n;x_h;k;x_l] h *)
+(* Not accepted yet *)
+
+(* reifiable *)
+(* val wallet_attack_loop : *)
+(*   h0:heap -> *)
+(*   n:id -> *)
+(*   vl:list id{List.length vl = 4 /\ List.noRepeats vl} -> *)
+(*   IntStore unit (requires (fun h -> h == h0 /\ List.hd vl == n)) *)
+(*     (ensures (fun _ _ _ -> True)) *)
+(*     (decreases (sel h0 n)) *)
+(* let rec wallet_attack_loop h0 n l = *)
+(*   assert (List.length l = 4) ; *)
+(*   match l with *)
+(*   | [n ; x_h ; k ; x_l] -> *)
+(*     let x = read n in *)
+(*     assert (sel h0 n == x) ; *)
+(*     if x > 0 then *)
+(*       write k (pow2 (x - 1)) ; *)
+(*       wallet [x_h;k;x_l] ; *)
+(*       write n (x - 1) ; *)
+(*       let h = IS?.get () in *)
+(*       assert (sel h n = x - 1) ; *)
+(*       wallet_attack_loop h n l *)
+(*   | _ -> () *)
 
 (* val wallet_attack : prog 4 *)
 (* let wallet_attack [n;x_h;k;x_l] h = *)
@@ -179,7 +218,7 @@ let sum [y ; x1 ; x2 ; x3 ; x4 ; x5] =
 (*  wallet_attack_loop [n;x_h;k;x_l] h *)
 
 (* (\* This does not verify, as expected *)
-(*    Howver, also does not verify wieht x_h : Low, which should be fine *\) *)
+(*    Howver, also does not verify with x_h : Low, which should be fine *\) *)
 (* (\* *)
 (* val verify_wallet_attack (n x_h k x_l : ref int): *)
 (*   Lemma *)
