examples/dm4free/FStar.DM4F.IntStoreFixed.fst
@@ -49,11 +49,11 @@ let write (i:id) (x:int)
   IS?.put (upd store i x)
 
 
-let read_does_not_write_lemma (h:heap) (x:id)
-  : Lemma (requires True)
-      (ensures (snd (reify (read x) h) == h))
-      [SMTPat (snd (reify (read x) h))]
-= ()
+(* let read_does_not_write_lemma (h:heap) (x:id) *)
+(*   : Lemma (requires True) *)
+(*       (ensures (snd (reify (read x) h) == h)) *)
+(*       [SMTPat (snd (reify (read x) h))] *)
+(* = () *)
 
 unfold
 let (!) = read
